\documentclass[11pt]{article}
\usepackage{import}
\input{../icml/latex-defs.tex}
\usepackage{fullpage}

\title{Quadratic Weights}
\author{Jacob Steinhardt}
\begin{document}
\maketitle
We are interested in the following learning problem: our experts 
consist of all vectors $w \geq 0$, $\|w\|_2 = 1$; our adversary 
can play any move $z_t$ with $z_t \leq 0$, $\|z_t\|_2 \leq \rho$. 
All vectors lie in $\bR^n$.
Our end goal is to obtain a regret bound that does not grow with $T$:
namely
\[ \sum_{t=1}^T w_t^Tx_t \leq \frac{2\rho \sqrt{n}}{\epsilon} + (1-\epsilon)\sum_{t=1}^T w^Tx_t, \]
for all experts $w$.

We will do this using the following updates:
\begin{align*}
        x_{1, i} &= 1,\ \forall i \\
        x_{t+1, i} &= \sqrt{x_{t,i}^2 - \eta x_{t,i}z_{t,i}} \\
        \Phi^{(t+1)} &= \sqrt{\sum_{i=1}^n x_{t+1,i}^2} \\
        w_{t+1,i} &= \frac{1}{\Phi^{(t+1)}}x_{t+1,i}
\end{align*}
The quantity $\Phi^{(t+1)}$ is a normalization constant used to 
ensure that $\|w_t\|_2 = 1$. We will use $(\Phi^{(t+1)})^2$ as a 
potential function to bound the regret:
\begin{align*}
        (\Phi^{(t+1)})^2 &= \sum_{i=1}^n x_{t+1,i}^2 \\
                         &= \sum_{i=1}^n x_{t,i}^2 - \eta x_{t,i}z_{t,i} \\
                         &= (\Phi^{(t)})^2 - \eta \Phi^{(t)}w_t^Tz_t \\
                         &\leq (\Phi^{(t)}-\frac{\eta}{2}w_t^Tz_t)^2.
\end{align*}
By induction we then obtain:
\begin{align}
        (\Phi^{(T+1)})^2 &\leq (\Phi^{(1)}-\frac{\eta}{2}\sum_{t=1}^Tw_t^Tz_t)^2 \\
                         &= (\sqrt{n}-\frac{\eta}{2}\sum_{t=1}^Tw_t^Tz_t)^2.
\end{align}

We next obtain a bound in the other direction; for this, we will need the 
inequality $\sqrt{1-x} \geq 1-\frac{x}{2}-\frac{x^2}{2}$ for $x \leq 1$.

We have:
\begin{align*}
        x_{t+1,i} &= \sqrt{x_{t,i}^2 - \eta x_{t,i}z_{t,i}} \\
                  &= x_{t,i}\sqrt{1-\eta\frac{z_{t,i}}{x_{t,i}}} \\
                  &\geq x_{t,i}(1-\frac{\eta}{2}\frac{z_{t,i}}{x_{t,i}} - \frac{\eta^2}{2}\frac{z_{t,i}^2}{x_{t,i}} \\
                  &\geq x_{t,i} - \frac{\eta}{2}z_{t,i} + \frac{\eta^2\rho}{2}z_{t,i},
\end{align*}
where in the last step we used the fact 
that $0 \geq z_{t,i} \geq -\rho$ and $x_{t,i} \geq 1$.

Again by induction, we have
\[ x_{T+1,i} \geq 1-\frac{\eta-\eta^2\rho}{2}\sum_{t=1}^T z_{t,i}. \]
Since $(\Phi^{(T+1)})^2 = \sum_{i=1}^n x_{T+1,i}^2$, we have, by combining 
the above inequality with our earlier upper bound:
\begin{align}
        (\sqrt{n}-\frac{\eta}{2}\sum_{t=1}^T w_t^Tz_t)^2 &\geq (\Phi^{(t+1)})^2 \\
                                                         &\geq \sum_{i=1}^n (1-\frac{\eta-\eta^2\rho}{2}\sum_{t=1}^T z_{t,i})^2 \\
                                                         &\geq (w^T1 - \sum_{t=1}^T w^Tz_t)^2.
\end{align}
We thus have:
\[ \frac{\eta}{2}\sum_{t=1}^T w_t^Tz_t \leq \sqrt{n} + \frac{\eta-\eta^2\rho}{2}\sum_{t=1}^T w^Tz_t. \]
Setting $\eta$ to $\frac{\epsilon}{\rho}$, we obtain
\[ \sum_{t=1}^T w_t^Tz_t \leq \frac{2\rho\sqrt{n}}{\epsilon} + (1-\epsilon)\sum_{t=1}^T w_t^Tz_t, \]
as was to be shown.

\end{document}
